---
title: "Weekly Problem 2: Harmonic, Geometric And Arithmetic Mean Inequality"
date: "2020-07-13"
tages: [Number Theory]
header:
  overlay_image: "/images/WeeklyP2/means.png"
  teaser: "/images/WeeklyP2/means.png"
TeX: {
  extensions: ["AMSmath.js", "AMSsymbols.js"]
}
excerpt: "Number Theory, Analysis"
mathjax: "true"
image:
  thumb: "/images/WeeklyP2/means.png"
---

## Theorem

This week the problem is one of the most beautiful proof that I have ever seen. There many proofs about this theorem, I will write here my favorite ones (in other words, I will write what I know).

Let $$x_1, x_2, x_3, ... , x_n \in \mathbb{R}^{+}$$. Then, HM (Harmonic mean) $$\leq$$ GM (Geometric mean) $$\leq$$ AM (arithmetic mean), in mathematical notation:

$$ \frac{n}{\frac{1}{x_1} + \frac{1}{x_2} + ... + \frac{1}{x_n}} \leq \sqrt[n]{x_1x_2...x_n} \leq \frac{x_1+x_2+...+x_n}{n}$$

, with equality in both cases if and only if all $$x_i$$â€™s are equal. Before we prove this, try to prove yourself.

## Proof 1

If you not familiar with mathematical induction see [1].
The proof 1 is showed by non-standard induction. Let $$P(n)$$ be the statement of the second inequality, in other words, written in the form as well as,

$$ x_1 x_2...x_n \leq \left(\frac{x_1+x_2+...+x_n}{n}\right)^{n}$$

For $$n=2$$, we have $$x_1 x_2 \leq \left(\frac{x_1+x_2}{2}\right)^{2} \iff (x_1 + x_2)^2 \geq 0$$, that is true. Now we have to show two things:

- **(1)** $$P(n) \implies P(n-1)$$
- **(2)** $$ P(n)$$ and $$P(2) \implies P(2n)$$

which will clearly show us the full result.

To prove **(1)**, let $$A = \sum_{k=1}^{n-1}\frac{x_k}{n-1}$$, then

$$\left(\prod_{k=1}^{n-1}x_k\right)A \overset{\mathrm{P(n)}}{\leq} \left(\frac{\sum_{k=1}^{n-1}x_k + A}{n}\right)^2$$

$$\;\;\;\;\;\;\;\;\;\;\;\;\;\;\;\;\;\;\;\;\;\;\;\;\;\;\;\;\;=\left(\frac{(n-1)A+A}{n}\right)^n = A^{n}$$

and hence,

$$\prod_{k=1}^{n-1}x_k \leq A^{n-1} = \left(\frac{\sum_{k=1}^{n-1}x_k}{n-1}\right)$$

To prove **(2)**, we see

$$\prod_{k=1}^{2n}x_k = \left(\prod_{k=1}^{n}x_k\right)\left(\prod_{k=n+1}^{2n}x_k\right)$$

$$\;\;\;\;\;\;\;\;\;\;\;\;\;\;\;\;\;\overset{\mathrm{P(n)}}{\leq}\left(\sum_{k=1}^{n}\frac{x_k}{n}\right)^n\left(\sum_{k=n+1}^{2n}\frac{x_k}{n}\right)^n$$

$$\;\;\;\overset{\mathrm{P(2)}}{\leq}\left(\frac{\sum_{k=1}^{2n}\frac{x_k}{n}}{2}\right)^{2n}$$

$$\;\;\; = \left(\frac{\sum_{k=1}^{2n}x_k}{2n}\right)^{2n}$$

The condition for equality is derived just as easily.

Now, let's prove the inequality $$ \frac{n}{\frac{1}{x_1} + \frac{1}{x_2} + ... + \frac{1}{x_n}} \leq \sqrt[n]{x_1x_2...x_n}$$. Actually it is a direct consequence of $$ x_1 x_2...x_n \leq \left(\frac{x_1+x_2+...+x_n}{n}\right)^{n}$$. Now, we will define a new set that is related to $$x_1, x_2, x_3, ... , x_n$$. $$y_j = \frac{1}{x_j}$$ for $$ j \in 1,2,..,n$$. So, our GM (geometric mean) - AM (Arithmetic Mean) becomes:

$$\sqrt[n]{\frac{1}{y_1 y_2...y_n}} \leq \frac{\frac{1}{y_1}+\frac{1}{y_2}+...+\frac{1}{y_n}}{n}$$
